More preparation for SSS >-> LTS.

HoareLogic/LocalTraceSemantics.v
@@ -9,33 +9,31 @@ Require Import Logic.HoareLogic.Trace.
 
 Class LocalTraceSemantics (P: ProgrammingLanguage) (state: Type): Type := {
   denote: cmd -> trace state -> Prop;
-  denote_defined: forall c s, exists tr, denote c tr /\ begin_state tr (Terminating s);
-  trace_non_empty: forall c tr, denote c tr -> ~ is_empty_stream tr;
-  trace_forward_legal: forall c tr n ms ms', denote c tr -> tr n = Some (ms, ms') -> ms <> NonTerminating /\ ms <> Error;
+  denote_defined: forall c s, exists tr, denote c tr /\ begin_state tr s;
   trace_sequential: forall c tr, denote c tr -> sequential_trace tr
 }.
 
 Definition access {P: ProgrammingLanguage} {state: Type} {LTS: LocalTraceSemantics P state} (s: state) (c: cmd) (ms: MetaState state) :=
-  exists tr, denote c tr /\ begin_state tr (Terminating s) /\ end_state tr ms.
+  exists tr, denote c tr /\ begin_end_state s tr ms.
 
 Class SALocalTraceSemantics (P: ProgrammingLanguage) (state: Type) {J: Join state} {kiM: KripkeIntuitionisticModel state} (LTS: LocalTraceSemantics P state): Type := {
   frame_property: forall c tr' m mf m',
     join m mf m' ->
     denote c tr' ->
-    begin_state tr' (Terminating m') ->
+    begin_state tr' m' ->
     exists tr,
     denote c tr /\
-    begin_state tr (Terminating m) /\
+    begin_state tr m /\
     (end_state tr Error \/
      exists trf,
        sequential_trace trf /\
-       begin_state trf (Terminating mf) /\
+       begin_state trf mf /\
        (forall k m' n',
          tr' k = Some (m', n') ->
          exists m n mf nf,
          tr k = Some (m, n) /\
          trf k = Some (mf, nf) /\
-         lift_Korder nf mf /\
+         lift_Korder nf (Terminating mf) /\
          lift_join n nf n'))
 }.
 
@@ -47,6 +45,8 @@ Export DT.
 Class ImpLocalTraceSemantics (P: ProgrammingLanguage) {iP: ImperativeProgrammingLanguage P} (state: Type) {kiM: KripkeIntuitionisticModel state} (LTS: LocalTraceSemantics P state): Type := {
   eval_bool: state -> bool_expr -> Prop;
   eval_bool_stable: forall b, Korder_stable (fun s => eval_bool s b);
+  denote_Sskip: forall tr,
+    denote Sskip tr -> is_empty_stream tr;
   denote_Ssequence: forall c1 c2 tr,
     denote (Ssequence c1 c2) tr ->
     traces_app (denote c1) (traces_app decrease_trace (denote c2)) tr;
@@ -68,7 +68,8 @@ Module Partial := ImpLocalTraceSemantics (ProgramState.Partial) (Trace.Partial).
 
 Instance Total2Partial_ImpLocalTraceSemantics {P: ProgrammingLanguage} {iP: ImperativeProgrammingLanguage P} (state: Type) {kiM: KripkeIntuitionisticModel state} {LTS: LocalTraceSemantics P state} (iLTS: Total.ImpLocalTraceSemantics P state LTS): Partial.ImpLocalTraceSemantics P state LTS.
 Proof.
-  refine (Partial.Build_ImpLocalTraceSemantics _ _ _ _ _ Total.eval_bool Total.eval_bool_stable _ _ _).
+  refine (Partial.Build_ImpLocalTraceSemantics _ _ _ _ _ Total.eval_bool Total.eval_bool_stable _ _ _ _).
+  + apply Total.denote_Sskip.
   + intros.
     pose proof Total.denote_Ssequence c1 c2 tr H.
     clear H; revert tr H0.
