HoareLogic/SimpleSmallStepSemantics.v
@@ -7,9 +7,9 @@ Class SimpleSmallStepSemantics (P: ProgrammingLanguage) (state: Type): Type := {
   simple_step: cmd * state -> cmd * state -> Prop
 }.
 
-Definition step {P: ProgrammingLanguage} {state: Type} {SSSS: SimpleSmallStepSemantics P state} (cs: cmd * state) (mcs: MetaState (cmd * state)) :=
+Definition step {P: ProgrammingLanguage} {state: Type} {SSSS: SimpleSmallStepSemantics P state} (final_state: cmd * state -> Prop) (cs: cmd * state) (mcs: MetaState (cmd * state)) :=
   match mcs with
   | Terminating cs0 => simple_step cs cs0
   | NonTerminating => False
-  | Error => forall cs0, ~ simple_step cs cs0
+  | Error => ~ final_state cs /\ forall cs0, ~ simple_step cs cs0
   end.
