lib/Stream/StreamSplit.v
@@ -1,0 +1,36 @@
+Require Import Coq.omega.Omega.
+Require Import Coq.Lists.List.
+Require Import Coq.Arith.Wf_nat.
+Require Import Logic.lib.Coqlib.
+Require Import Logic.lib.Stream.SigStream.
+Require Import Logic.lib.Stream.SigStream.
+Require Import Logic.lib.Stream.StreamFunctions.
+
+Lemma cut2_exists {A: Type}: forall (h: stream A) (P: A -> Prop),
+  (exists h1 h2,
+     h = stream_app h1 h2 /\
+     (forall n a, h1 n = Some a -> ~ P a) /\
+     (exists a, h2 0 = Some a /\ P a)) \/
+  (forall n a, h n = Some a -> ~ P a).
+Proof.
+  intros.
+  destruct (classic (exists n a, h n = Some a /\ P a)).
+  + left.
+    apply (dec_inh_nat_subset_has_unique_least_element
+             _ (fun n => classic _)) in H.
+    destruct H as [n [[? ?] _]].
+    destruct H as [a [? ?]].
+    exists (fstn_stream n h), (skipn_stream n h).
+    split; [| split].
+    - symmetry; apply stream_app_fstn_skipn.
+    - clear H H1 a.
+      intros; intro.
+      destruct (lt_dec n0 n);
+        [| rewrite fstn_stream_None in H by omega; congruence].
+      rewrite fstn_stream_Some in H by auto.
+      specialize (H0 n0 (ex_intro _ a (conj H H1))).
+      omega.
+    - exists a; split; auto.
+  + right.
+    firstorder.
+Qed.
